Unify typing.

AOT_semantics.thy
@@ -230,13 +230,16 @@ specification (AOT_lambda0)
   AOT_sem_lambda0: "AOT_lambda0 \<phi> = \<phi>"
   by (rule_tac x="\<lambda>x. x" in exI) simp
 
-specification(AOT_concrete)
-  AOT_sem_concrete: \<open>[w \<Turnstile> E!\<kappa>] = AOT_model_concrete w \<kappa>\<close>
-  AOT_sem_concrete_denotes: \<open>[w \<Turnstile> E!\<down>]\<close>
+consts AOT_sem_concrete :: \<open><'a::AOT_UnaryIndividualTerm>\<close>
+specification(AOT_sem_concrete)
+  AOT_sem_concrete: \<open>AOT_model_valid_in w (AOT_exe AOT_sem_concrete \<kappa>) = AOT_model_concrete w \<kappa>\<close>
+  AOT_sem_concrete_denotes: \<open>AOT_model_valid_in w (AOT_denotes AOT_sem_concrete)\<close>
   by (rule_tac x=\<open>Abs_rel (\<lambda> x . \<epsilon>\<^sub>\<o> w . AOT_model_concrete w x)\<close> in exI)
      (auto simp: AOT_model_no_special_nondenoting AOT_model_concrete_denotes AOT_model_concrete_equiv AOT_model_regular_\<kappa>_def
                  AOT_model_proposition_choice_simp AOT_sem_exe Abs_rel_inverse AOT_model_denotes_rel_def AOT_sem_denotes)
-
+specification(AOT_concrete)
+  AOT_concrete_sem: \<open>\<guillemotleft>E!\<guillemotright> = AOT_sem_concrete\<close>
+  by simp
 
 
 lemma AOT_sem_equiv_defI:
@@ -301,12 +304,12 @@ lemma AOT_sem_id_def0E3:
   using AOT_sem_id_def0E1[OF assms]
   by (simp add: AOT_sem_eq AOT_sem_denotes)
 
-lemma AOT_sem_ordinary_def_denotes: \<open>[w \<Turnstile> [\<lambda>x \<diamond>E!x]\<down>]\<close>
+lemma AOT_sem_ordinary_def_denotes: \<open>[w \<Turnstile> [\<lambda>x \<diamond>[\<guillemotleft>AOT_sem_concrete\<guillemotright>]x]\<down>]\<close>
   unfolding AOT_sem_denotes AOT_model_lambda_denotes
-  by (auto simp: AOT_sem_dia AOT_model_concrete_equiv AOT_sem_concrete AOT_sem_denotes)
-lemma AOT_sem_abstract_def_denotes: \<open>[w \<Turnstile> [\<lambda>x \<not>\<diamond>E!x]\<down>]\<close>
+  by (auto simp: AOT_sem_dia AOT_concrete_sem AOT_model_concrete_equiv AOT_sem_concrete AOT_sem_denotes)
+lemma AOT_sem_abstract_def_denotes: \<open>[w \<Turnstile> [\<lambda>x \<not>\<diamond>[\<guillemotleft>AOT_sem_concrete\<guillemotright>]x]\<down>]\<close>
   unfolding AOT_sem_denotes AOT_model_lambda_denotes
-  by (auto simp: AOT_sem_dia AOT_model_concrete_equiv AOT_sem_concrete AOT_sem_denotes AOT_sem_not)
+  by (auto simp: AOT_sem_dia AOT_concrete_sem AOT_model_concrete_equiv AOT_sem_concrete AOT_sem_denotes AOT_sem_not)
 
 class AOT_Individual = 
   fixes AOT_sem_proj_id :: \<open>'a::AOT_IndividualTerm \<Rightarrow> ('a \<Rightarrow> \<o>) \<Rightarrow> ('a \<Rightarrow> \<o>) \<Rightarrow> \<o>\<close>
@@ -517,12 +520,12 @@ end
 
 class AOT_UnaryEnc = AOT_UnaryIndividualTerm +
   assumes AOT_sem_enc_eq: \<open>[v \<Turnstile> \<Pi>\<down> & \<Pi>'\<down> & \<box>\<forall>\<nu> (\<nu>[\<Pi>] \<equiv> \<nu>[\<Pi>']) \<rightarrow> \<Pi> = \<Pi>']\<close>
-      and AOT_sem_a_objects: \<open>[v \<Turnstile> \<exists>x (\<not>\<diamond>E!x & \<forall>F (x[F] \<equiv> \<phi>{F}))]\<close>
+      and AOT_sem_a_objects: \<open>[v \<Turnstile> \<exists>x (\<not>\<diamond>[\<guillemotleft>AOT_sem_concrete\<guillemotright>]x & \<forall>F (x[F] \<equiv> \<phi>{F}))]\<close>
       and AOT_sem_unary_proj_enc: \<open>AOT_proj_enc x \<psi> = AOT_enc x \<guillemotleft>[\<lambda>z \<psi>{z}]\<guillemotright>\<close>
-      and AOT_sem_nocoder: \<open>[v \<Turnstile> E!\<kappa>] \<Longrightarrow> \<not>[w \<Turnstile> \<guillemotleft>AOT_enc \<kappa> \<Pi>\<guillemotright>]\<close>
+      and AOT_sem_nocoder: \<open>[v \<Turnstile> [\<guillemotleft>AOT_sem_concrete\<guillemotright>]\<kappa>] \<Longrightarrow> \<not>[w \<Turnstile> \<guillemotleft>AOT_enc \<kappa> \<Pi>\<guillemotright>]\<close>
       and AOT_sem_ind_eq: \<open>([v \<Turnstile> \<kappa>\<down>] \<and> [v \<Turnstile> \<kappa>'\<down>] \<and> \<kappa> = \<kappa>') =
-       (([v \<Turnstile> [\<lambda>x \<diamond>E!x]\<kappa>] \<and> [v \<Turnstile> [\<lambda>x \<diamond>E!x]\<kappa>'] \<and> (\<forall> v \<Pi> . [v \<Turnstile> \<Pi>\<down>] \<longrightarrow> [v \<Turnstile> [\<Pi>]\<kappa>] = [v \<Turnstile> [\<Pi>]\<kappa>']))
-      \<or> ([v \<Turnstile> [\<lambda>x \<not>\<diamond>E!x]\<kappa>] \<and> [v \<Turnstile> [\<lambda>x \<not>\<diamond>E!x]\<kappa>'] \<and> (\<forall> v \<Pi> . [v \<Turnstile> \<Pi>\<down>] \<longrightarrow> [v \<Turnstile> \<kappa>[\<Pi>]] = [v \<Turnstile> \<kappa>'[\<Pi>]])))\<close>
+       (([v \<Turnstile> [\<lambda>x \<diamond>[\<guillemotleft>AOT_sem_concrete\<guillemotright>]x]\<kappa>] \<and> [v \<Turnstile> [\<lambda>x \<diamond>[\<guillemotleft>AOT_sem_concrete\<guillemotright>]x]\<kappa>'] \<and> (\<forall> v \<Pi> . [v \<Turnstile> \<Pi>\<down>] \<longrightarrow> [v \<Turnstile> [\<Pi>]\<kappa>] = [v \<Turnstile> [\<Pi>]\<kappa>']))
+      \<or> ([v \<Turnstile> [\<lambda>x \<not>\<diamond>[\<guillemotleft>AOT_sem_concrete\<guillemotright>]x]\<kappa>] \<and> [v \<Turnstile> [\<lambda>x \<not>\<diamond>[\<guillemotleft>AOT_sem_concrete\<guillemotright>]x]\<kappa>'] \<and> (\<forall> v \<Pi> . [v \<Turnstile> \<Pi>\<down>] \<longrightarrow> [v \<Turnstile> \<kappa>[\<Pi>]] = [v \<Turnstile> \<kappa>'[\<Pi>]])))\<close>
 
 instantiation \<kappa> :: AOT_Enc
 begin
@@ -592,24 +595,24 @@ instance proof
     using AOT_meta_a_objects_\<kappa> by fastforce
 next
   fix v and \<phi>:: \<open><\<kappa>> \<Rightarrow> \<o>\<close>
-  show \<open>[v \<Turnstile> \<exists>x (\<not>\<diamond>E!x & \<forall>F (x[F] \<equiv> \<phi>{F}))]\<close>
+  show \<open>[v \<Turnstile> \<exists>x (\<not>\<diamond>[\<guillemotleft>AOT_sem_concrete\<guillemotright>]x & \<forall>F (x[F] \<equiv> \<phi>{F}))]\<close>
     using AOT_model_a_objects[of "\<lambda> \<Pi> . [v \<Turnstile> \<phi>{\<Pi>}]"]
     by (auto simp: AOT_sem_denotes AOT_sem_exists AOT_sem_conj AOT_sem_not AOT_sem_dia AOT_sem_concrete AOT_enc_\<kappa>_meta AOT_sem_equiv AOT_sem_forall)
 next
   show \<open>AOT_proj_enc x \<psi> = AOT_enc x (AOT_lambda \<psi>)\<close> for x :: \<kappa> and \<psi>
     by (simp add: AOT_proj_enc_\<kappa>_def)
 next
-  show \<open>[v \<Turnstile> E!\<kappa>] \<Longrightarrow> \<not> [w \<Turnstile> \<kappa>[\<Pi>]]\<close> for v w and \<kappa> :: \<kappa> and \<Pi>
+  show \<open>[v \<Turnstile> [\<guillemotleft>AOT_sem_concrete\<guillemotright>]\<kappa>] \<Longrightarrow> \<not> [w \<Turnstile> \<kappa>[\<Pi>]]\<close> for v w and \<kappa> :: \<kappa> and \<Pi>
     by (simp add: AOT_enc_\<kappa>_meta AOT_sem_concrete AOT_model_nocoder)
 next
-  let ?ordeq = \<open>\<lambda>v \<kappa> \<kappa>'. [v \<Turnstile> [\<lambda>x \<diamond>E!x]\<kappa>] \<and> [v \<Turnstile> [\<lambda>x \<diamond>E!x]\<kappa>'] \<and> (\<forall> v \<Pi> . AOT_model_denotes \<Pi> \<longrightarrow> [v \<Turnstile> [\<Pi>]\<kappa>] = [v \<Turnstile> [\<Pi>]\<kappa>'])\<close>
-  let ?abseq = \<open>\<lambda>v \<kappa> \<kappa>'. [v \<Turnstile> [\<lambda>x \<not>\<diamond>E!x]\<kappa>] \<and> [v \<Turnstile> [\<lambda>x \<not>\<diamond>E!x]\<kappa>'] \<and> (\<forall> v \<Pi> . AOT_model_denotes \<Pi> \<longrightarrow> [v \<Turnstile> \<kappa>[\<Pi>]] = [v \<Turnstile> \<kappa>'[\<Pi>]])\<close>
+  let ?ordeq = \<open>\<lambda>v \<kappa> \<kappa>'. [v \<Turnstile> [\<lambda>x \<diamond>[\<guillemotleft>AOT_sem_concrete\<guillemotright>]x]\<kappa>] \<and> [v \<Turnstile> [\<lambda>x \<diamond>[\<guillemotleft>AOT_sem_concrete\<guillemotright>]x]\<kappa>'] \<and> (\<forall> v \<Pi> . AOT_model_denotes \<Pi> \<longrightarrow> [v \<Turnstile> [\<Pi>]\<kappa>] = [v \<Turnstile> [\<Pi>]\<kappa>'])\<close>
+  let ?abseq = \<open>\<lambda>v \<kappa> \<kappa>'. [v \<Turnstile> [\<lambda>x \<not>\<diamond>[\<guillemotleft>AOT_sem_concrete\<guillemotright>]x]\<kappa>] \<and> [v \<Turnstile> [\<lambda>x \<not>\<diamond>[\<guillemotleft>AOT_sem_concrete\<guillemotright>]x]\<kappa>'] \<and> (\<forall> v \<Pi> . AOT_model_denotes \<Pi> \<longrightarrow> [v \<Turnstile> \<kappa>[\<Pi>]] = [v \<Turnstile> \<kappa>'[\<Pi>]])\<close>
   fix v and \<kappa> \<kappa>' :: \<kappa>
   {
     assume 0: \<open>[v \<Turnstile> \<kappa>\<down>] \<and> [v \<Turnstile> \<kappa>'\<down>] \<and> \<kappa> = \<kappa>'\<close>
     {
       assume \<open>is_\<omega>\<kappa> \<kappa>'\<close>
-      hence \<open>[v \<Turnstile> [\<lambda>x \<diamond>E!x]\<kappa>']\<close>
+      hence \<open>[v \<Turnstile> [\<lambda>x \<diamond>[\<guillemotleft>AOT_sem_concrete\<guillemotright>]x]\<kappa>']\<close>
         apply (subst AOT_sem_lambda_beta[OF AOT_sem_ordinary_def_denotes, of v \<kappa>'])
          apply (simp add: "0")
         apply (simp add: AOT_sem_dia)
@@ -618,7 +621,7 @@ next
     }
     moreover {
       assume \<open>is_\<alpha>\<kappa> \<kappa>'\<close>
-      hence \<open>[v \<Turnstile> [\<lambda>x \<not>\<diamond>E!x]\<kappa>']\<close>
+      hence \<open>[v \<Turnstile> [\<lambda>x \<not>\<diamond>[\<guillemotleft>AOT_sem_concrete\<guillemotright>]x]\<kappa>']\<close>
         apply (subst AOT_sem_lambda_beta[OF AOT_sem_abstract_def_denotes, of v \<kappa>'])
          apply (simp add: "0")
         apply (simp add: AOT_sem_not AOT_sem_dia)
@@ -648,7 +651,7 @@ next
     hence \<kappa>_denotes: \<open>[v \<Turnstile> \<kappa>\<down>]\<close> and \<kappa>'_denotes: \<open>[v \<Turnstile> \<kappa>'\<down>]\<close> 
       by (simp add: AOT_sem_denotes AOT_sem_exe)+
     hence \<open>\<not>is_\<omega>\<kappa> \<kappa>\<close> and \<open>\<not>is_\<omega>\<kappa> \<kappa>'\<close>
-      by (metis AOT_model_\<omega>_concrete_in_some_world AOT_model_concrete_\<kappa>.simps(1) AOT_sem_concrete AOT_sem_dia AOT_sem_exe AOT_sem_lambda_beta AOT_sem_not \<kappa>.collapse(1) \<open>[v \<Turnstile> [\<lambda>x \<not>\<diamond>E!x]\<kappa>] \<and> [v \<Turnstile> [\<lambda>x \<not>\<diamond>E!x]\<kappa>'] \<and> (\<forall>v \<Pi>. AOT_model_denotes \<Pi> \<longrightarrow> [v \<Turnstile> \<kappa>[\<Pi>]] = [v \<Turnstile> \<kappa>'[\<Pi>]])\<close>)+
+      by (metis AOT_model_\<omega>_concrete_in_some_world AOT_model_concrete_\<kappa>.simps(1) AOT_sem_concrete AOT_sem_dia AOT_sem_exe AOT_sem_lambda_beta AOT_sem_not \<kappa>.collapse(1) \<open>[v \<Turnstile> [\<lambda>x \<not>\<diamond>[\<guillemotleft>AOT_sem_concrete\<guillemotright>]x]\<kappa>] \<and> [v \<Turnstile> [\<lambda>x \<not>\<diamond>[\<guillemotleft>AOT_sem_concrete\<guillemotright>]x]\<kappa>'] \<and> (\<forall>v \<Pi>. AOT_model_denotes \<Pi> \<longrightarrow> [v \<Turnstile> \<kappa>[\<Pi>]] = [v \<Turnstile> \<kappa>'[\<Pi>]])\<close>)+
     hence \<open>is_\<alpha>\<kappa> \<kappa>\<close> and \<open>is_\<alpha>\<kappa> \<kappa>'\<close>
       by (meson AOT_sem_denotes AOT_model_denotes_\<kappa>_def \<kappa>.exhaust_disc \<kappa>_denotes \<kappa>'_denotes)+
     then obtain x y where \<kappa>_def: "\<kappa> = \<alpha>\<kappa> x" and \<kappa>'_def: "\<kappa>' = \<alpha>\<kappa> y"
@@ -663,7 +666,7 @@ next
         apply (simp add: AOT_model_denotes_\<kappa>_def)
         by (metis (mono_tags) AOT_rel_equiv_def Quotient_def urrel_quotient)
       hence \<open>[v \<Turnstile> \<kappa>'[\<guillemotleft>urrel_to_rel r\<guillemotright>]]\<close>
-        using AOT_enc_\<kappa>_meta \<open>[v \<Turnstile> [\<lambda>x \<not>\<diamond>E!x]\<kappa>] \<and> [v \<Turnstile> [\<lambda>x \<not>\<diamond>E!x]\<kappa>'] \<and> (\<forall>v \<Pi>. AOT_model_denotes \<Pi> \<longrightarrow> [v \<Turnstile> \<kappa>[\<Pi>]] = [v \<Turnstile> \<kappa>'[\<Pi>]])\<close> by blast
+        using AOT_enc_\<kappa>_meta \<open>[v \<Turnstile> [\<lambda>x \<not>\<diamond>[\<guillemotleft>AOT_sem_concrete\<guillemotright>]x]\<kappa>] \<and> [v \<Turnstile> [\<lambda>x \<not>\<diamond>[\<guillemotleft>AOT_sem_concrete\<guillemotright>]x]\<kappa>'] \<and> (\<forall>v \<Pi>. AOT_model_denotes \<Pi> \<longrightarrow> [v \<Turnstile> \<kappa>[\<Pi>]] = [v \<Turnstile> \<kappa>'[\<Pi>]])\<close> by blast
       hence \<open>r \<in> y\<close>
         unfolding \<kappa>'_def
         unfolding AOT_enc_\<kappa>_meta
@@ -681,7 +684,7 @@ next
         apply (simp add: AOT_model_denotes_\<kappa>_def)
         by (metis (mono_tags) AOT_rel_equiv_def Quotient_def urrel_quotient)
       hence \<open>[v \<Turnstile> \<kappa>[\<guillemotleft>urrel_to_rel r\<guillemotright>]]\<close>
-        using AOT_enc_\<kappa>_meta \<open>[v \<Turnstile> [\<lambda>x \<not>\<diamond>E!x]\<kappa>] \<and> [v \<Turnstile> [\<lambda>x \<not>\<diamond>E!x]\<kappa>'] \<and> (\<forall>v \<Pi>. AOT_model_denotes \<Pi> \<longrightarrow> [v \<Turnstile> \<kappa>[\<Pi>]] = [v \<Turnstile> \<kappa>'[\<Pi>]])\<close> by blast
+        using AOT_enc_\<kappa>_meta \<open>[v \<Turnstile> [\<lambda>x \<not>\<diamond>[\<guillemotleft>AOT_sem_concrete\<guillemotright>]x]\<kappa>] \<and> [v \<Turnstile> [\<lambda>x \<not>\<diamond>[\<guillemotleft>AOT_sem_concrete\<guillemotright>]x]\<kappa>'] \<and> (\<forall>v \<Pi>. AOT_model_denotes \<Pi> \<longrightarrow> [v \<Turnstile> \<kappa>[\<Pi>]] = [v \<Turnstile> \<kappa>'[\<Pi>]])\<close> by blast
       hence \<open>r \<in> x\<close>
         unfolding \<kappa>_def
         unfolding AOT_enc_\<kappa>_meta
@@ -694,8 +697,8 @@ next
       using \<kappa>'_def \<kappa>'_denotes \<kappa>_def by blast
   }
   ultimately show \<open>([v \<Turnstile> \<kappa>\<down>] \<and> [v \<Turnstile> \<kappa>'\<down>] \<and> \<kappa> = \<kappa>') =
-       (([v \<Turnstile> [\<lambda>x \<diamond>E!x]\<kappa>] \<and> [v \<Turnstile> [\<lambda>x \<diamond>E!x]\<kappa>'] \<and> (\<forall> v \<Pi> . [v \<Turnstile> \<Pi>\<down>] \<longrightarrow> [v \<Turnstile> [\<Pi>]\<kappa>] = [v \<Turnstile> [\<Pi>]\<kappa>']))
-      \<or> ([v \<Turnstile> [\<lambda>x \<not>\<diamond>E!x]\<kappa>] \<and> [v \<Turnstile> [\<lambda>x \<not>\<diamond>E!x]\<kappa>'] \<and> (\<forall> v \<Pi> . [v \<Turnstile> \<Pi>\<down>] \<longrightarrow> [v \<Turnstile> \<kappa>[\<Pi>]] = [v \<Turnstile> \<kappa>'[\<Pi>]])))\<close>
+       (([v \<Turnstile> [\<lambda>x \<diamond>[\<guillemotleft>AOT_sem_concrete\<guillemotright>]x]\<kappa>] \<and> [v \<Turnstile> [\<lambda>x \<diamond>[\<guillemotleft>AOT_sem_concrete\<guillemotright>]x]\<kappa>'] \<and> (\<forall> v \<Pi> . [v \<Turnstile> \<Pi>\<down>] \<longrightarrow> [v \<Turnstile> [\<Pi>]\<kappa>] = [v \<Turnstile> [\<Pi>]\<kappa>']))
+      \<or> ([v \<Turnstile> [\<lambda>x \<not>\<diamond>[\<guillemotleft>AOT_sem_concrete\<guillemotright>]x]\<kappa>] \<and> [v \<Turnstile> [\<lambda>x \<not>\<diamond>[\<guillemotleft>AOT_sem_concrete\<guillemotright>]x]\<kappa>'] \<and> (\<forall> v \<Pi> . [v \<Turnstile> \<Pi>\<down>] \<longrightarrow> [v \<Turnstile> \<kappa>[\<Pi>]] = [v \<Turnstile> \<kappa>'[\<Pi>]])))\<close>
     unfolding AOT_sem_denotes
     by auto
 qed
@@ -797,15 +800,15 @@ no_notation AOT_abstract ("\<^bold>A\<^bold>!")
 end
 
 lemma AOT_sem_ordinary: "\<guillemotleft>O!\<guillemotright> = \<guillemotleft>[\<lambda>x \<diamond>E!x]\<guillemotright>"
-  using AOT_ordinary[THEN AOT_sem_id_def0E1, OF AOT_sem_ordinary_def_denotes]
+  using AOT_ordinary[THEN AOT_sem_id_def0E1]  AOT_sem_ordinary_def_denotes AOT_concrete_sem
   by (auto simp: AOT_sem_eq)
 lemma AOT_sem_abstract: "\<guillemotleft>A!\<guillemotright> = \<guillemotleft>[\<lambda>x \<not>\<diamond>E!x]\<guillemotright>"
-  using AOT_abstract[THEN AOT_sem_id_def0E1, OF AOT_sem_abstract_def_denotes]
+  using AOT_abstract[THEN AOT_sem_id_def0E1]  AOT_sem_abstract_def_denotes AOT_concrete_sem
   by (auto simp: AOT_sem_eq)
 lemma AOT_sem_ordinary_denotes: \<open>[w \<Turnstile> O!\<down>]\<close>
-  by (simp add: AOT_sem_ordinary AOT_sem_ordinary_def_denotes)
+  by (simp add: AOT_sem_ordinary AOT_sem_ordinary_def_denotes AOT_concrete_sem)
 lemma AOT_meta_abstract_denotes: \<open>[w \<Turnstile> A!\<down>]\<close>
-  by (simp add: AOT_sem_abstract AOT_sem_abstract_def_denotes)
+  by (simp add: AOT_sem_abstract AOT_sem_abstract_def_denotes AOT_concrete_sem)
 
 (********* TODO: this is still a mess - simplify all this and make sure it's valid ********)
 definition AOT_instance_of_cqt_2 :: \<open>('a::AOT_\<kappa>s \<Rightarrow> \<o>) \<Rightarrow> bool\<close> where
@@ -964,5 +967,8 @@ AOT_theorem prod_denotesE: assumes \<open>\<guillemotleft>(\<kappa>\<^sub>1,\<ka
   using assms by (simp add: AOT_sem_denotes AOT_sem_conj AOT_model_denotes_prod_def)
 AOT_theorem prod_denotesI: assumes \<open>\<kappa>\<^sub>1\<down> & \<kappa>\<^sub>2\<down>\<close> shows \<open>\<guillemotleft>(\<kappa>\<^sub>1,\<kappa>\<^sub>2)\<guillemotright>\<down>\<close>
   using assms by (simp add: AOT_sem_denotes AOT_sem_conj AOT_model_denotes_prod_def)
+
+AOT_register_type_constraints
+  Individual: \<open>\<kappa>\<close> \<open>_::AOT_\<kappa>s\<close>
 
 end
